LeanModels/Es.lean
@@ -7,6 +7,7 @@ import LeanModels.Es.Object
 import LeanModels.Es.Ordinary
 import LeanModels.Es.Env
 import LeanModels.Es.Function
+import LeanModels.Es.Convert
 import LeanModels.Es.SpecAttr
 import LeanModels.Es.Spec
 
